$$
  \left[ {\begin{array}{cc}
   1 & 0 \\
   0 & -1 \\
  \end{array} } \right]
$$

$$
  \left[ {\begin{array}{cc}
   -1 & 0 \\
   0 & 1 \\
  \end{array} } \right]
$$
$$
  \frac{1}{m^2+1}
  \left[ {\begin{array}{cc}
   1-m^2 & 2m \\
   2m & m^2-1 \\
  \end{array} } \right]
$$
$$
  \left[ {\begin{array}{cc}
   cos\theta & -sin\theta \\
   sin\theta & cos\theta \\
  \end{array} } \right]
$$
$$
  \left[ {\begin{array}{cc}
   cos\theta & sin\theta \\
   -sin\theta & cos\theta \\
  \end{array} } \right]
$$

$$
S_\phi \circ T_\theta \sim
  \left[ {\begin{array}{cc}
   cos(\phi + \theta) & -sin(\phi +\theta) \\
   sin(\phi +\theta) & cos(\phi +\theta) \\
  \end{array} } \right]
$$
$$
S_{\phi} \circ T_{\theta} = \left[ {\begin{array}{cc} cos(\phi + \theta) & sin(\phi +\theta) \\ -sin(\phi +\theta) & cos(\phi +\theta) \\ \end{array} } \right]
$$
$$
\frac{Z_1}{Z_2}=(\frac{x_1x_2+y_1y_2}{x_2^2+y_2^2}, \frac{x_2y_1-x_1y_2}{x_2^2+y_2^2})
$$
$$
Z^{-1}=(\frac{x}{x^2+y^2},\frac{-y}{x^2+y^2})
$$
$$
\frac{Z_1}{Z_2} = (\frac{r_1}{r_2}cos(\theta_1-\theta_2), \frac{r_1}{r_2}sin(\theta_1-\theta_2)
$$

$\overline Z = (x, -y)$
$\overline {Z+Z} = \overline Z_1 + \overline Z_2$
$Z^{-1} = \frac{\overline{Z}}{|Z|^2}$
$Z\overline Z = |Z|^2$
Re(Z) = $\frac{Z+\overline{Z}}{2}$
Im(Z) = $\frac{Z-\overline{Z}}{2i}$

$e^{i\theta}=cos\theta + isin\theta$
$e^{i\theta_1}e^{i\theta_2} = e^{i(\theta_1+\theta_2)}$
$\overline {e^{i\theta}} = e^{-i\theta}$
$(e^{i\theta})^{-1} = e^{-i\theta}$
